a more refined algorithm for the reduction Is_to_Vc - an example how to use a foreach loop

TSTSC_Poly.thy
@@ -1,7 +1,7 @@
 theory TSTSC_Poly
   imports "NREST.NREST" Three_Sat_To_Set_Cover  "Landau_Symbols.Landau_More"
-  "NREST.RefineMonadicVCG"
-begin
+  "NREST.RefineMonadicVCG" "NREST.Refine_Foreach"
+begin                             
 
 
 
@@ -31,26 +31,72 @@ definition "ispolyred c A B ma mb = (\<exists>f p ps. \<forall>pi. c pi \<le> SP
                               \<and>  (\<forall>pi. mb (f pi) \<le> ps (ma pi))
                                    \<and> poly p \<and> poly ps \<and> is_reduction f A B )" 
 
+definition "ispolyredd c RI RO A B ma mb = (\<exists>f p ps. \<forall>pi pi'. ((pi',pi):RI \<longrightarrow>  c pi' \<le> \<Down>RO (SPEC (\<lambda>y. y = f pi) (\<lambda>_. p (ma pi))))
+                              \<and>  (\<forall>pi. mb (f pi) \<le> ps (ma pi))
+                                   \<and> poly p \<and> poly ps \<and> is_reduction f A B )" 
 
+thm SPEC_def
+lemma ispolyredd_generalizes_ispolyred:
+  "ispolyred c A B ma mb = ispolyredd c Id Id A B ma mb"
+  unfolding ispolyred_def ispolyredd_def by auto
 
-lemma ispolyred_trans:
-  assumes 1: "ispolyred c1 A B ma mb"
-    and 2: "ispolyred c2 B C mb mc"
+lemma ispolyredd_generalizes_ispolyredD:
+  "ispolyred c A B ma mb \<Longrightarrow> ispolyredd c Id Id A B ma mb"
+  using ispolyredd_generalizes_ispolyred ..
+  
+
+thm conc_fun_chain  
+
+lemma ispolyredd_refine:
+  assumes 
+    1: "ispolyredd c1 RA RB A B ma mb" 
+      and 2: "\<And>pi' pi''. (pi'',pi')\<in>RA' \<Longrightarrow>  c' pi'' \<le> \<Down>RB' (c1 pi')"
   shows 
-      "ispolyred (\<lambda>a. bind (c1 a) c2) A C ma mc"
+    "ispolyredd c' (RA' O RA) (RB' O RB) A B ma mb"
 proof -
   from 1 obtain f1 p1 ps1 where
-     spec1: "\<And>pi. c1 pi \<le> SPEC (\<lambda>y. y = f1 pi) (\<lambda>_.  (p1 (ma pi)))"
+     spec1: "\<And>pi pi'. (pi',pi)\<in>RA \<Longrightarrow> c1 pi' \<le> \<Down>RB (SPEC (\<lambda>y. y = f1 pi) (\<lambda>_.  (p1 (ma pi))))"
    and size1: "\<And>pi. mb (f1 pi) \<le> ps1 (ma pi)"
-    and p1: "poly p1" "poly ps1" and "is_reduction f1 A B" unfolding ispolyred_def by blast
+    and p1: "poly p1" "poly ps1" and "is_reduction f1 A B" unfolding ispolyredd_def by blast
+
+
+  show ?thesis
+    unfolding ispolyredd_def
+    apply(rule exI[where x=f1])
+    apply(rule exI[where x=p1])
+    apply(rule exI[where x=ps1])
+    apply safe
+    subgoal  apply(rule order.trans)
+       apply(rule 2) apply simp
+      apply(rule order.trans)
+       apply(rule nrest_Rel_mono) 
+      apply(rule spec1) apply simp
+      apply(subst conc_fun_chain) by simp
+    subgoal by fact
+    subgoal by fact
+    subgoal by fact
+    subgoal by fact
+    done
+qed
+
+lemma ispolyredd_trans:
+  assumes 1: "ispolyredd c1 RA RB A B ma mb"
+    and 2: "ispolyredd c2 RB RC B C mb mc"
+  shows 
+      "ispolyredd (\<lambda>a. bind (c1 a) c2) RA RC A C ma mc"
+proof -
+  from 1 obtain f1 p1 ps1 where
+     spec1: "\<And>pi pi'. (pi',pi)\<in>RA \<Longrightarrow> c1 pi' \<le> \<Down>RB (SPEC (\<lambda>y. y = f1 pi) (\<lambda>_.  (p1 (ma pi))))"
+   and size1: "\<And>pi. mb (f1 pi) \<le> ps1 (ma pi)"
+    and p1: "poly p1" "poly ps1" and "is_reduction f1 A B" unfolding ispolyredd_def by blast
 
   from 2 obtain f2 p2 ps2 where
-      spec2: "\<And>pi. c2 pi \<le> SPEC (\<lambda>y. y = f2 pi) (\<lambda>_. enat (p2 (mb pi)))"
+      spec2: "\<And>pi pi'. (pi',pi)\<in>RB \<Longrightarrow> c2 pi' \<le> \<Down>RC (SPEC (\<lambda>y. y = f2 pi) (\<lambda>_. enat (p2 (mb pi))))"
     and size2: "\<And>pi. mc (f2 pi) \<le> ps2 (mb pi)"
-     and p2: "poly p2" "poly ps2" "is_reduction f2 B C" unfolding ispolyred_def by blast
+     and p2: "poly p2" "poly ps2" "is_reduction f2 B C" unfolding ispolyredd_def by blast
 
-  thm spec1[unfolded SPEC_def, THEN T_specifies_rev]
-  thm spec2[unfolded SPEC_def, THEN T_specifies_rev]
+  thm spec1[unfolded SPEC_def ]
+  thm spec2[unfolded SPEC_def ]
 
   then obtain p2' where p2'_ub: "\<And>x. p2 x \<le> p2' x" and p2'_poly: "poly p2'"
     and   p2'_mono: "\<And>i j. i\<le>j \<Longrightarrow> p2' i \<le> p2' j" 
@@ -62,16 +108,19 @@ proof -
  
 
   show ?thesis
-    unfolding ispolyred_def
+    unfolding ispolyredd_def
     apply(rule exI[where x="f2 o f1"])
     apply(rule exI[where x="\<lambda>n. p1 n + p2' (ps1 n)"])
     apply(rule exI[where x="\<lambda>n. ps2' (ps1 n)"])
     apply safe
     subgoal unfolding SPEC_def
-  apply(rule T_specifies_I)
-      apply(vcg' \<open>-\<close> rules: spec1[unfolded SPEC_def, THEN T_specifies_rev, THEN T_conseq4]
-  spec2[unfolded SPEC_def, THEN T_specifies_rev, THEN T_conseq4]
-        )
+      apply(rule order.trans)
+       apply(rule bindT_refine)
+      apply (rule spec1) apply simp
+       apply (rule spec2) apply simp
+      apply(rule nrest_Rel_mono)  
+  apply(rule T_specifies_I)  
+      apply(vcg' \<open>-\<close> rules: T_SPEC )
       apply (auto split: if_splits)
       subgoal apply(rule order_trans[OF p2'_ub]) using size1 p2'_mono  
         by auto   
@@ -86,15 +135,27 @@ proof -
       apply(rule is_reduction_trans) by fact+ 
     done
 qed
-  
 
+
+lemma ispolyred_trans:
+  "ispolyred c1 A B ma mb \<Longrightarrow> ispolyred c2 B C mb mc
+    \<Longrightarrow> ispolyred (\<lambda>a. bind (c1 a) c2) A C ma mc"
+  using ispolyredd_generalizes_ispolyred ispolyredd_trans by metis
+    
 
 definition "size_IS = (\<lambda>(E,k). card E)"
 definition "size_VC = (\<lambda>(E,k). card E)"
 
 section "IS to VC"
 
-definition "mop_get_vertices_card E = REST [(card (\<Union> E)) \<mapsto> card E]"
+subsection \<open>A trivial implementation\<close>
+
+text \<open>Here we assume that we have an operation that returns
+      the size of the set of vertices.\<close>
+
+definition "mop_get_vertices_card E = REST [(card (\<Union> E)) \<mapsto> 2 * card E + 2]"
+
+text \<open>Then we can easily give an abstract algorithm for the reduction:\<close>
 
 definition "is_to_vc = (\<lambda>(E,k). 
           do {
@@ -105,7 +166,7 @@ definition "is_to_vc = (\<lambda>(E,k).
               RETURNT (E, s-k)
           })"
 
-definition "vc_time n = n" 
+definition "vc_time n = 2 * n + 2" 
 definition "vc_space n = n" 
 
 
@@ -124,8 +185,9 @@ lemma is_to_vc_size:
 thm is_reduction_is_vc
 
 
-term vertex_cover
-lemma "ispolyred is_to_vc independent_set vertex_cover size_IS size_VC" 
+text \<open>And we show that it actually is a polynomial reduction:\<close>
+
+lemma is_to_vc_ispolyred: "ispolyred is_to_vc independent_set vertex_cover size_IS size_VC" 
   unfolding ispolyred_def
   apply(rule exI[where x=is_vc])
   apply(rule exI[where x=vc_time])
@@ -133,14 +195,157 @@ lemma "ispolyred is_to_vc independent_set vertex_cover size_IS size_VC"
   apply(safe)
   subgoal using is_to_vc_refines by blast
   subgoal using is_to_vc_size  by blast 
-  subgoal unfolding poly_def vc_time_def apply(rule exI[where x=1]) by simp
+  subgoal unfolding poly_def vc_time_def apply(rule exI[where x=1]) by auto
   subgoal unfolding poly_def vc_space_def apply(rule exI[where x=1]) by simp
   subgoal using is_reduction_is_vc .
   done
 
 
 
+subsection \<open>A more fine grained algorith\<close>
 
+text \<open>now we assume to only have more fine grained basic operations.\<close>
+
+text \<open>This setup is actually unrealistic, it is hard to imagine a datastructure with
+  constant insertion and constant cardinality query.
+     TODO: make cost of insert linear in size of S\<close>
+
+definition "mop_set_insert S s = REST [insert s S \<mapsto> 1]"
+
+definition "mop_set_card S  = REST [card S \<mapsto> 1]"
+
+definition "mop_set_empty_set = REST [ {} \<mapsto> 1]"
+
+
+text \<open>Now we want to work on lists of tuples to represent the Edge set:\<close>
+
+definition "R_edge_set_tuple_list = {(xs,E) |xs E. ((\<lambda>(a,b). {a,b}) ` (set xs) = E \<and> distinct xs
+           \<and> inj_on (\<lambda>(a,b). {a,b}) (set xs)  )}"
+text \<open>here the constraint @{term inj_on} means, that the edge list xs
+       does not contain any loops ( (a,a) ),
+        or both symmetric edges ( (a,b)\<in>set xs \<and> (b,a)\<in>set xs )\<close> 
+
+
+text \<open>we can restate the specification to get the cardinality of the set of vertices given
+      an edge list, and that it refines the operation @{term mop_get_vertices_card}\<close>
+
+definition "mop_get_vertices_card' xs = REST [(card (\<Union> ((\<lambda>(a,b). {a,b}) ` (set xs)))) \<mapsto> 2 * length xs + 2]"
+
+lemma mop_get_vertices_card_data_refine:  
+  assumes "(xs,E)\<in>R_edge_set_tuple_list"
+  shows "mop_get_vertices_card' xs \<le> mop_get_vertices_card E"
+proof -
+  from assms have E: "E = (\<lambda>(a,b). {a,b}) ` (set xs)"
+     and *: "distinct xs""inj_on (\<lambda>(a,b). {a,b}) (set xs)"
+    unfolding R_edge_set_tuple_list_def by auto
+  have **: "card E = length xs" 
+    by(simp add: card_image distinct_card E *)
+  show ?thesis    
+    unfolding mop_get_vertices_card'_def mop_get_vertices_card_def
+    unfolding ** by(simp add: E)
+qed
+
+text \<open>now let's implement getting the cardinality of V with the basic set operations\<close>
+
+definition get_vertices_card :: "('b*'b) list \<Rightarrow> nat nrest" where
+  "get_vertices_card es = do {
+      S \<leftarrow> mop_set_empty_set;
+      S' \<leftarrow> nfoldli es (\<lambda>_. True) 
+            (\<lambda>(a,b) S. do {
+                  S \<leftarrow> mop_set_insert S a;
+                  S \<leftarrow> mop_set_insert S b;
+                  RETURNT S }) 
+
+        S;
+      n \<leftarrow> mop_set_card S';
+      RETURNT n
+    }"
+ 
+
+lemma get_vertices_card_refine:
+  "get_vertices_card xs \<le> mop_get_vertices_card' xs"
+proof -
+  let ?I = "\<lambda>(xs::('b*'b)list) ys (S::'b set).  S = \<Union> ((\<lambda>(a,b). {a,b}) ` (set xs))"
+
+  show ?thesis
+  unfolding get_vertices_card_def mop_get_vertices_card'_def
+  apply(rule T_specifies_I)
+  apply(subst nfoldliIE_def[symmetric, where I="?I" and E=2])
+  unfolding mop_set_empty_set_def
+  apply(vcg' -) 
+  apply(rule nfoldliIE_rule[THEN T_specifies_rev, THEN T_conseq4, where P2="?I xs []" ])
+       apply simp
+  subgoal 
+    apply(rule T_specifies_I)
+    unfolding mop_set_insert_def
+    apply(vcg' -)
+    apply auto unfolding Some_le_emb'_conv
+    by auto
+     apply simp
+    apply simp
+  apply (rule order.refl)
+  unfolding mop_set_card_def
+  apply (vcg' -) apply auto unfolding Some_le_emb'_conv Some_eq_emb'_conv
+   apply (auto simp add: one_enat_def)    
+  done 
+qed
+
+lemma get_vertices_card_data_refine:
+  assumes "(xs,E)\<in>R_edge_set_tuple_list"
+  shows "get_vertices_card xs \<le>  (mop_get_vertices_card E)"
+  apply(rule order.trans) 
+  apply(rule   get_vertices_card_refine)
+  apply(rule mop_get_vertices_card_data_refine)
+  by fact
+
+text \<open>now we can give a refined algorithm, only using the fine grained operations:\<close>
+
+definition "is_to_vc2 = (\<lambda>(xs,k). 
+          do {
+            s \<leftarrow> get_vertices_card xs;
+            if k > s  then
+              RETURNT (xs,k)
+            else
+              RETURNT (xs, s-k)
+          })"
+
+
+lemma R_reintro: "A \<le>   B \<Longrightarrow> A \<le> \<Down>Id B" by simp
+
+term " prod_rel R_edge_set_tuple_list Id"
+lemma is_to_vc2_refines:
+  "((xs,k),(E,k)) \<in> R_edge_set_tuple_list \<times>\<^sub>r Id
+     \<Longrightarrow> is_to_vc2 (xs,k) \<le> \<Down> (R_edge_set_tuple_list \<times>\<^sub>r Id) (is_to_vc (E,k))"
+  unfolding is_to_vc_def is_to_vc2_def
+  apply (refine_rcg get_vertices_card_data_refine[THEN R_reintro] )
+  subgoal by (auto simp: prod_rel_def_internal)
+  subgoal by (auto simp: prod_rel_def_internal)
+  subgoal by (auto simp: RETURNT_refine prod_rel_def_internal)
+  subgoal by(auto intro!: RETURNT_refine simp: prod_rel_def_internal)
+  done
+lemma is_to_vc2_refines':
+  "(i',i) \<in> R_edge_set_tuple_list \<times>\<^sub>r Id
+     \<Longrightarrow> is_to_vc2 i' \<le> \<Down> (R_edge_set_tuple_list \<times>\<^sub>r Id) (is_to_vc i)"
+  unfolding is_to_vc_def is_to_vc2_def
+  apply (refine_rcg get_vertices_card_data_refine[THEN R_reintro] )
+  subgoal by (auto simp: prod_rel_def_internal)
+  subgoal by (auto simp: prod_rel_def_internal)
+  subgoal by (auto simp: RETURNT_refine prod_rel_def_internal)
+  subgoal by(auto intro!: RETURNT_refine simp: prod_rel_def_internal)
+  done
+
+
+thm ispolyredd_refine[OF is_to_vc_ispolyred[THEN ispolyredd_generalizes_ispolyredD] is_to_vc2_refines' ]
+    is_to_vc2_refines
+
+text \<open>Finally we can show that the new algorithm also is a polynomial reduction acting on 
+      lists of tuples instead of an abstract edge set\<close>
+
+lemma "ispolyredd is_to_vc2
+       (R_edge_set_tuple_list \<times>\<^sub>r nat_rel) (R_edge_set_tuple_list \<times>\<^sub>r nat_rel)
+        independent_set vertex_cover size_IS size_VC"
+  apply(rule ispolyredd_refine[OF is_to_vc_ispolyred[THEN ispolyredd_generalizes_ispolyredD], simplified])
+  apply(rule is_to_vc2_refines' ) .
 
 
 
